more reorg

theories/iris/allocator/reprs.v
@@ -7,37 +7,12 @@ From iris.bi Require Export weakestpre.
 From Wasm.iris.logrel Require Export iris_fundamental.
 From Wasm.iris.rules Require Export proofmode.
 From RWasm.iris.allocator Require Import allocator_common misc_relocate.
-
-Definition mem_block_at_pos_frac `{!wasmG Σ} (q: dfrac) (n: N) (l:bytes) k : iProp Σ :=
-  ([∗ list] i ↦ b ∈ l, n ↦[wm]{q} [ (N.of_nat (N.to_nat k+i)) ] b)%I.
-Locate "↦[wms][".
-
-Notation "n ↦[wms]{ q } [ i ] l" := (mem_block_at_pos_frac q n l i)                    
-                                      (at level 20, q at level 5, format "n ↦[wms]{ q } [ i ] l"): bi_scope.
+From RWasm.iris.allocator Require Export blocks memrsc.
+Import blocks.
 
 Section reprs.
 
 Context `{!wasmG Σ}. 
-
-Inductive state_flag :=
-| Used
-| Free
-| Final.
-
-Inductive block : Type :=
-| UsedBlk
-    (blk_used_size: N)
-    (blk_leftover_size: N)
-    (*(blk_padding: iProp Σ)*)
-| FreeBlk
-    (blk_size: N).
-
-Inductive final_block : Type :=
-| FinalBlk
-    (blk_size: N).
-
-Definition blocks : Type :=
-  list block * final_block.
 
 (* beware:
     The i32 type is a record {intval: Z; proof: -1 < z < 2^32}.
@@ -81,23 +56,6 @@ Proof.
     + lia.
 Qed.
 
-Definition block_flag blk :=
-  match blk with
-  | UsedBlk _ _ => Used
-  | FreeBlk _ => Free
-  end.
-
-Definition final_block_flag blk :=
-  match blk with
-  | FinalBlk _ => Final
-  end.
-
-Definition block_size blk : N :=
-  match blk with
-  | UsedBlk sz_u sz_l => sz_u + sz_l
-  | FreeBlk sz => sz
-  end.
-
 Definition state_to_N (flag : state_flag) : N :=
   match flag with
   | Used => BLK_USED
@@ -111,59 +69,6 @@ Definition state_frac flag : Qp :=
   | _ => 1
   end.
 
-Lemma mem_block_at_frac_one n i l :
-  n ↦[wms]{DfracOwn 1}[i] l ⊢ n ↦[wms][i] l.
-Proof.
-  iIntros.
-  iFrame.
-Qed.
-    
-
-Lemma mem_block_at_frac_combine n p q i l l' :
-  n ↦[wms]{p}[i] l ∗ n ↦[wms]{q}[i] l' ⊢ n ↦[wms]{p ⋅ q}[i] l ∗ ⌜l = l'⌝.
-Proof.
-Admitted.
-
-Lemma mem_block_at_frac_split n p q i l :
-  n ↦[wms]{p ⋅ q}[i] l ⊢
-  n ↦[wms]{p}[i] l ∗ n ↦[wms]{q}[i] l.
-Proof.
-Admitted.
-
-Lemma mem_block_at_frac_halve n i l :
-  n ↦[wms][i] l ⊢
-  n ↦[wms]{DfracOwn (1/2)}[i] l ∗ n ↦[wms]{DfracOwn (1/2)}[i] l.
-Proof.
-  iIntros "H".
-  iApply mem_block_at_frac_split.
-  rewrite dfrac_op_own.
-  rewrite Qp.half_half.
-  iFrame.
-Qed.
-
-Definition own_vec (memidx: N) (base_addr: N) (sz: N) : iProp Σ :=
-  ∃ bs: bytes, ⌜N.of_nat (length bs) = sz⌝ ∗ memidx ↦[wms][base_addr] bs.
-
-Definition own_half_vec (memidx: N) (base_addr: N) (sz: N) : iProp Σ :=
-  ∃ bs: bytes, ⌜N.of_nat (length bs) = sz⌝ ∗ memidx ↦[wms]{DfracOwn (1/2)}[base_addr] bs.
-
-Lemma own_half_vec_split memidx base_addr sz:
-  own_half_vec memidx base_addr sz ∗ own_half_vec memidx base_addr sz ⊣⊢ own_vec memidx base_addr sz.
-Proof.
-  iSplit.
-  - iIntros "[[%b [%len H]] [%b' [%len' H']]]".
-    iPoseProof (mem_block_at_frac_combine with "[$]") as "[Hcomb %Hbeq]".
-    subst b'.
-    rewrite dfrac_op_own.
-    rewrite Qp.half_half.
-    iExists b.
-    by iFrame.
-  - iIntros "(%b & %bsz & H)".
-    iPoseProof (mem_block_at_frac_halve with "[$]") as "[Hp Hq]".
-    by iFrame.
-Qed.
-
-Eval vm_compute in bits (VAL_int32 (Wasm_int.Int32.repr (Z.of_N (state_to_N Used)))).
 Definition alloc_tok (memidx: N) (data_addr: N) : iProp Σ :=
   ∃ st,
     ⌜N_repr (state_to_N Used) st⌝ ∗
