theories/iris/allocator/blocks.v
@@ -1,0 +1,38 @@
+Require Import Coq.NArith.BinNat.
+
+Inductive state_flag :=
+| Used
+| Free
+| Final.
+
+Inductive block : Type :=
+| UsedBlk
+    (blk_used_size: N)
+    (blk_leftover_size: N)
+    (*(blk_padding: iProp Σ)*)
+| FreeBlk
+    (blk_size: N).
+
+Inductive final_block : Type :=
+| FinalBlk
+    (blk_size: N).
+
+Definition blocks : Type :=
+  list block * final_block.
+
+Definition block_flag blk :=
+  match blk with
+  | UsedBlk _ _ => Used
+  | FreeBlk _ => Free
+  end.
+
+Definition final_block_flag blk :=
+  match blk with
+  | FinalBlk _ => Final
+  end.
+
+Definition block_size blk : N :=
+  match blk with
+  | UsedBlk sz_u sz_l => sz_u + sz_l
+  | FreeBlk sz => sz
+  end.
